deps/poulet4/lib/P4automata/Benchmarks/IPOptions2Proof.v
@@ -1,0 +1,112 @@
+Require Import Poulet4.P4automata.Benchmarks.ProofHeader.
+Require Import Poulet4.P4automata.Benchmarks.IPOptions.
+Require Import Poulet4.P4automata.Benchmarks.Timestamp.
+
+Notation H := (IPOptionsRef62.header + TimestampSpec2.header).
+Notation A := (Sum.sum IPOptionsRef62.aut TimestampSpec2.aut).
+Notation conf := (P4automaton.configuration (P4A.interp A)).
+Notation start_left := IPOptionsRef62.Parse0.
+Notation start_right := TimestampSpec2.Parse0.
+
+Notation r_state_depth := 5.
+
+Definition r_states :=
+  Eval vm_compute in (Reachability.reachable_states
+                        A
+                        r_state_depth
+                        start_left
+                        start_right).
+
+(* Definition r_states' := 
+  Eval vm_compute in (Reachability.reachable_step r_states).
+
+Definition r_len := Eval vm_compute in (length r_states, length r_states').
+
+Print r_len. *)
+
+Definition top : Relations.rel conf := fun _ _ => True.
+Definition top' : Relations.rel (state_template A) := fun _ _ => True.
+
+Declare ML Module "mirrorsolve".
+
+RegisterEnvCtors
+  (IPOptionsRef62.T0, FirstOrderConfRelSimplified.Bits 8)
+  (IPOptionsRef62.L0, FirstOrderConfRelSimplified.Bits 8)
+  (IPOptionsRef62.V0, FirstOrderConfRelSimplified.Bits 48)
+  (IPOptionsRef62.T1, FirstOrderConfRelSimplified.Bits 8)
+  (IPOptionsRef62.L1, FirstOrderConfRelSimplified.Bits 8)
+  (IPOptionsRef62.V1, FirstOrderConfRelSimplified.Bits 48)
+  (IPOptionsRef62.Scratch8, FirstOrderConfRelSimplified.Bits 8)
+  (IPOptionsRef62.Scratch16, FirstOrderConfRelSimplified.Bits 16)
+  (IPOptionsRef62.Scratch24, FirstOrderConfRelSimplified.Bits 24)
+  (IPOptionsRef62.Scratch32, FirstOrderConfRelSimplified.Bits 32)
+  (IPOptionsRef62.Scratch40, FirstOrderConfRelSimplified.Bits 40)
+
+  (TimestampSpec2.T0, FirstOrderConfRelSimplified.Bits 8)
+  (TimestampSpec2.L0, FirstOrderConfRelSimplified.Bits 8)
+  (TimestampSpec2.V0, FirstOrderConfRelSimplified.Bits 48)
+  (TimestampSpec2.T1, FirstOrderConfRelSimplified.Bits 8)
+  (TimestampSpec2.L1, FirstOrderConfRelSimplified.Bits 8)
+  (TimestampSpec2.V1, FirstOrderConfRelSimplified.Bits 48)
+  (TimestampSpec2.Scratch8, FirstOrderConfRelSimplified.Bits 8)
+  (TimestampSpec2.Scratch16, FirstOrderConfRelSimplified.Bits 16)
+  (TimestampSpec2.Scratch24, FirstOrderConfRelSimplified.Bits 24)
+  (TimestampSpec2.Scratch32, FirstOrderConfRelSimplified.Bits 32)
+  (TimestampSpec2.Scratch40, FirstOrderConfRelSimplified.Bits 40)
+  (TimestampSpec2.Pointer, FirstOrderConfRelSimplified.Bits 8)
+  (TimestampSpec2.Overflow, FirstOrderConfRelSimplified.Bits 4)
+  (TimestampSpec2.Flag, FirstOrderConfRelSimplified.Bits 4)
+  (TimestampSpec2.Timestamp, FirstOrderConfRelSimplified.Bits 32).
+
+  Lemma prebisim_incremental_sep:
+  forall q1 q2,
+    interp_conf_rel' {| cr_st := {|
+                        cs_st1 := {|
+                          st_state := inl (inl (start_left));
+                          st_buf_len := 0;
+                        |};
+                        cs_st2 := {|
+                          st_state := inl (inr (start_right));
+                          st_buf_len := 0;
+                        |};
+                      |};
+                      cr_ctx := BCEmp;
+                      cr_rel := btrue;
+                   |} q1 q2 ->
+  pre_bisimulation A
+                   (wp r_states)
+                   top
+                   []
+                   (mk_init _ _ _ A r_state_depth start_left start_right)
+                   q1 q2.
+Proof.
+  idtac "running timestamp three bisimulation".
+  
+  intros.
+  set (a := A).
+  set (rel0 := (mk_init _ _ _ _ _ _ _)).
+  vm_compute in rel0.
+  subst rel0.
+
+  set (eight := 8).
+  assert (H8 : 8 = eight); [subst eight; reflexivity|].
+  set (sixteen := (Datatypes.S( Datatypes.S( Datatypes.S( Datatypes.S( Datatypes.S( Datatypes.S( Datatypes.S( Datatypes.S eight))))))))).
+  assert (H16 : (Datatypes.S( Datatypes.S( Datatypes.S( Datatypes.S( Datatypes.S( Datatypes.S( Datatypes.S( Datatypes.S eight)))))))) = sixteen); [subst sixteen; reflexivity|].
+  
+
+  try rewrite H8;
+  try rewrite H16;
+
+
+  match goal with 
+  | |- pre_bisimulation _ _ _ _ ?R _ _ => 
+    hashcons_list R
+  end.
+
+  time "build phase" repeat (run_bisim top top' r_states;
+    try rewrite H8;
+    try rewrite H16
+  ).
+  time "close phase" close_bisim top'.
+
+Time Admitted.
